Many updates and improvements

old/SemOld.v
@@ -1,10 +1,8 @@
 Require Import
-  Coq.ZArith.ZArith
   Hask.Control.Monad
   Hask.Data.Either
   ilist
   Lib
-  Ltac
   Ty
   Exp
   Value
@@ -19,25 +17,33 @@ Section Sem.
 
 Import ListNotations.
 
-Definition SemPrimType (ty : PrimType) : Set :=
-  match ty with
-  | PrimInteger => Z
-  | PrimDecimal => N
-  | PrimTime    => nat
-  | PrimBool    => bool
-  | PrimString  => string
-  | PrimUnit    => unit
-  end.
-
-Fixpoint SemTy (τ : Ty) : Set :=
+Fixpoint SemTy `{HostExprs A} (τ : Ty) : Type :=
   match τ with
-  | TyPrim ty       => SemPrimType ty
+  | TyPrim ty        => SemPrimType ty
   | TyList τ        => list (SemTy τ)
   | TyPair t1 t2    => SemTy t1 * SemTy t2
   | TyArrow dom cod => SemTy dom → Err + SemTy cod
+  (* | TyArrow dom cod => SemTy dom → SemTy cod *)
   end.
 
-Definition SemEnv Γ : Set := ilist SemTy Γ.
+Class HostExprsSem (A : Type) : Type := {
+  has_host_exprs :> HostExprs A;
+  (* HostExpSem {τ} : HostExp τ → Err + SemTy τ; *)
+  HostExpSem {τ} : HostExp τ → SemTy τ;
+
+  (* HostExpSem_valid {ty} (e : HostExp ty) : *)
+  (*   ∃ x, HostExpSem e = pure x; *)
+
+  CallHost {Γ dom cod} :
+    HostExp (dom ⟶ cod) → ∀ v : Exp Γ dom, ValueP v → Exp Γ cod;
+
+  Reduce {Γ τ} : HostExp τ → { v : Exp Γ τ & ValueP v };
+}.
+
+Context {A : Type}.
+Context `{HostExprsSem A}.
+
+Definition SemEnv Γ : Type := ilist SemTy Γ.
 
 Fixpoint SemVar `(v : Var Γ τ) : SemEnv Γ → SemTy τ :=
   match v with
@@ -98,38 +104,42 @@ Definition liftJoin2 `{Monad m} `(f : a -> b -> m c)
            (ma : m a) (mb : m b) : m c :=
    join (liftA2 f ma mb).
 
-Program Fixpoint SemExp `(e : Exp Γ τ) : SemEnv Γ → Err + SemTy τ :=
+Fixpoint SemExp `(e : Exp Γ τ) : SemEnv Γ → Err + SemTy τ :=
   match e with
+  (* | HostedExp x   => λ _,  HostExpSem x *)
+  (* | HostedVal x   => λ _,  HostExpSem x *)
+  (* | HostedFun x   => λ _,  HostExpSem x *)
   | Error e       => λ _,  inl e
-  | Lit l         => λ _,  inl Err_CarNil (* jww (2022-07-18): TODO *)
-  | Bltn b        => λ _,  inl Err_CarNil (* jww (2022-07-18): TODO *)
-  | If b t e      => λ se, b' <- SemExp b se ;
-                           SemExp (if b' : bool
-                                   then t
-                                   else e) se
-  | Pair x y      => λ se, liftA2 pair (SemExp x se) (SemExp y se)
-  | Fst p         => λ se, fst <$> SemExp p se
-  | Snd p         => λ se, snd <$> SemExp p se
-  | Nil           => λ se, pure nil
-  | Cons x xs     => λ se, x'  <- SemExp x se ;
-                           xs' <- SemExp xs se ;
-                           pure (x' :: xs')
-  | Car xs        => λ se, xs' <- SemExp xs se ;
-                           match xs' with
-                           | []     => inl Err_CarNil
-                           | x :: _ => pure x
-                           end
-  | Cdr xs        => λ se, xs' <- SemExp xs se ;
-                           match xs' with
-                           | []      => inl Err_CdrNil
-                           | _ :: xs => pure xs
-                           end
-  | IsNil xs      => λ se, xs' <- SemExp xs se ;
-                           pure (match xs' with
-                                 | []      => true
-                                 | _ :: xs => false
-                                 end)
-  | Seq exp1 exp2 => λ se, SemExp exp1 se >> SemExp exp2 se
+  | EUnit         => λ _,  pure tt
+  (* | ETrue         => λ _,  pure true *)
+  (* | EFalse        => λ _,  pure false *)
+  (* | If b t e      => λ se, b' <- SemExp b se ; *)
+  (*                          SemExp (if b' : bool *)
+  (*                                  then t *)
+  (*                                  else e) se *)
+  (* | Pair x y      => λ se, liftA2 prod (SemExp x se) (SemExp ys se) *)
+  (* | Fst p         => λ se, fst <$> SemExp p se *)
+  (* | Snd p         => λ se, snd <$> SemExp p se *)
+  (* | Nil           => λ se, pure nil *)
+  (* | Cons x xs     => λ se, x'  <- SemExp x se ; *)
+  (*                          xs' <- SemExp xs se ; *)
+  (*                          pure (x' :: xs') *)
+  (* | Car xs        => λ se, xs' <- SemExp xs se ; *)
+  (*                          match xs' with *)
+  (*                          | []     => inl CarOfNil *)
+  (*                          | x :: _ => pure x *)
+  (*                          end *)
+  (* | Cdr xs        => λ se, xs' <- SemExp xs se ; *)
+  (*                          pure (match xs' with *)
+  (*                                | []      => nil *)
+  (*                                | _ :: xs => xs *)
+  (*                                end) *)
+  (* | IsNil xs      => λ se, xs' <- SemExp xs se ; *)
+  (*                          pure (match xs' with *)
+  (*                                | []      => true *)
+  (*                                | _ :: xs => false *)
+  (*                                end) *)
+  (* | Seq exp1 exp2 => λ se, SemExp exp1 se >> SemExp exp2 se *)
 
   | VAR v         => λ se, pure (SemVar v se)
   | LAM e         => λ se, pure (λ x, SemExp e (x, se))
@@ -139,23 +149,21 @@ Program Fixpoint SemExp `(e : Exp Γ τ) : SemEnv Γ → Err + SemTy τ :=
 Definition sem `(e : Exp [] τ) : Err + SemTy τ := SemExp e tt.
 Arguments sem {_} _ /.
 
+(*
 Lemma SemExp_RenSem {Γ Γ' τ} (e : Exp Γ τ) (r : Ren Γ' Γ) (se : SemEnv Γ') :
   SemExp e (RenSem r se) = SemExp (RenExp r e) se.
 Proof.
   generalize dependent Γ'.
   induction e; simpl; intros; auto.
-  - rewrite IHe1; repeat f_equal.
-    extensionality b.
-    now destruct b; simpl.
-  - rewrite IHe2; repeat f_equal.
-    now apply IHe1.
-  - now rewrite IHe.
-  - now rewrite IHe.
-  - now rewrite IHe1, IHe2.
-  - now rewrite IHe.
-  - now rewrite IHe.
-  - now rewrite IHe.
-  - now rewrite IHe1, IHe2.
+  (* - now rewrite IHe1, IHe2, IHe3. *)
+  (* - now rewrite IHe1, IHe2. *)
+  (* - now rewrite IHe. *)
+  (* - now rewrite IHe. *)
+  (* - now rewrite IHe1, IHe2. *)
+  (* - now rewrite IHe. *)
+  (* - now rewrite IHe. *)
+  (* - now rewrite IHe. *)
+  (* - now rewrite IHe1, IHe2. *)
   - now rewrite SemVar_RenSem.
   - f_equal.
     extensionality z.
@@ -180,13 +188,22 @@ Lemma SemExp_ValueP {Γ τ} (e : Exp Γ τ) (se : SemEnv Γ) :
 Proof.
   induction 1; simpl; intros;
   try (now eexists; eauto); reduce.
-  - admit.                      (* jww (2022-07-18): TODO *)
-  - admit.                      (* jww (2022-07-18): TODO *)
-  - exists (x1, x0).
-    now rewrite H1, H2; simpl.
-  - exists (x1 :: x0).
-    now rewrite H1, H2; simpl.
-Abort.
+Qed.
+(*
+  - pose proof (HostExpSem_valid x).
+    reduce.
+    rewrite H0.
+    now eexists.
+  - pose proof (HostExpSem_valid f).
+    reduce.
+    rewrite H0.
+    now eexists.
+  - rewrite H0, H1; simpl.
+    now eexists.
+  - rewrite H0, H1; simpl.
+    now eexists.
+Qed.
+*)
 
 (************************************************************************
  * SubSem
@@ -282,7 +299,7 @@ Qed.
 *)
 
 (*
-Inductive SubSem {Γ Γ'} (s : Sub Γ Γ') (se : SemEnv Γ) : SemEnv Γ' → Set :=
+Inductive SubSem {Γ Γ'} (s : Sub Γ Γ') (se : SemEnv Γ) : SemEnv Γ' → Type :=
   SubSem NoSub      _  := inr tt;
   SubSem (Push t σ) se := t' <- SemExp t se ;
                           ρ' <- SubSem σ se ;
@@ -391,6 +408,7 @@ Proof.
   dependent elimination s; simp RcS; simp SubSem; simp RenSem.
   now rewrite IHr.
 Qed.
+*)
 *)
 
 End Sem.
