src/Ty.v
@@ -8,49 +8,68 @@ Set Equations With UIP.
 
 Section Ty.
 
-Class HostTypes (A : Type) : Type := {
-  HostTy : Type;
-  HostTySem : HostTy → Type
-}.
+Inductive PrimType : Set :=
+  | PrimInteger
+  | PrimDecimal
+  | PrimTime
+  | PrimBool
+  | PrimString
+  | PrimUnit.
 
-Context {A : Type}.
-Context `{HostTypes A}.
+Derive NoConfusion NoConfusionHom Subterm EqDec for PrimType.
 
-(* TODO:
- - Row-types
- - Modules
- - Schemas
- - Tables
- - Guards
- - Capabilities *)
+Inductive Ty : Set :=
+  | TyPrim : PrimType → Ty
 
-Inductive Ty : Type :=
-  (* | TyHost : HostTy → Ty *)
+  | TyList : Ty → Ty
+  | TyPair : Ty → Ty → Ty
 
-  | TyUnit : Ty
-  (* | TyBool : Ty *)
-  (* | TyList : Ty → Ty *)
-  (* | TyPair : Ty → Ty → Ty *)
+  (* | TyCap : Ty → Ty → Ty *)
 
   (* The arrow type is the only type in the base lambda calculus *)
   | TyArrow : Ty → Ty → Ty.
 
-(* Derive NoConfusion NoConfusionHom EqDec Subterm for Ty. *)
-Derive NoConfusion NoConfusionHom EqDec for Ty.
+Derive NoConfusion NoConfusionHom Subterm EqDec for Ty.
+
+Inductive DecidableP : Ty → Set :=
+  | PrimDecP {ty} : DecidableP (TyPrim ty)
+  | ListDecP {τ} : DecidableP τ → DecidableP (TyList τ)
+  | PairDecP {τ1 τ2} : DecidableP τ1 → DecidableP τ2 →
+                       DecidableP (TyPair τ1 τ2).
+
+Derive Signature NoConfusion NoConfusionHom EqDec for DecidableP.
+
+Lemma DecidableP_irrelevance {τ} (H1 H2 : DecidableP τ) :
+  H1 = H2.
+Proof.
+  dependent induction H1;
+  dependent elimination H2; auto;
+  f_equal; congruence.
+Qed.
+
+Lemma DecidableP_dec {τ} :
+  DecidableP τ + (DecidableP τ → False).
+Proof.
+  induction τ; try solve [now left; constructor|now right].
+  - destruct IHτ.
+    + now left; constructor.
+    + right; intro; inversion H; contradiction.
+  - destruct IHτ1, IHτ2.
+    + now left; constructor.
+    + right; intro; inversion H; contradiction.
+    + right; intro; inversion H; contradiction.
+    + right; intro; inversion H; contradiction.
+Qed.
 
 End Ty.
 
-(* Arguments Ty {A H}. *)
-(* Arguments TyHost {A H} _. *)
-(* Arguments TyUnit {A H}. *)
-(* Arguments TyBool {A H}. *)
-(* Arguments TyList {A H} _. *)
-(* Arguments TyPair {A H} _ _. *)
-(* Arguments TyArrow {A H} _ _. *)
+Arguments PrimDecP.
+Arguments ListDecP {τ} _.
+Arguments PairDecP {τ1 τ2} _ _.
 
 Declare Scope Ty_scope.
 Bind Scope Ty_scope with Ty.
 Delimit Scope Ty_scope with ty.
 
 Infix "⟶" := TyArrow (at level 51, right associativity) : Ty_scope.
-(* Infix "×"  := TyPair  (at level 40, left associativity) : Ty_scope. *)
+Infix "×"  := TyPair  (at level 40, left associativity) : Ty_scope.
