src/Value.v
@@ -1,5 +1,6 @@
 Require Import
   Lib
+  Ltac
   Ty
   Exp.
 
@@ -12,25 +13,20 @@ Section Value.
 
 Import ListNotations.
 
-Context {A : Type}.
-Context `{HostExprs A}.
-
 Open Scope Ty_scope.
+
+Unset Elimination Schemes.
 
 (* [ValueP] is an inductive proposition that indicates whether an expression
    represents a value, i.e., that it does reduce any further. *)
 Inductive ValueP Γ : ∀ {τ}, Exp Γ τ → Prop :=
-  (* | HostedValP {ty} (x : HostExp (TyHost ty)) : ValueP Γ (HostedVal x) *)
-  (* | HostedFunP {dom cod} (f : HostExp (dom ⟶ cod)) : ValueP Γ (HostedFun f) *)
-  (* | ErrorP {τ} m : ValueP Γ (Error (τ:=τ) m) *)
-  | UnitP        : ValueP Γ EUnit
-  (* | TrueP        : ValueP Γ ETrue *)
-  (* | FalseP       : ValueP Γ EFalse *)
-  (* | PairP {τ1 τ2} {x : Exp Γ τ1} {y : Exp Γ τ2} : *)
-  (*   ValueP Γ x → ValueP Γ y → ValueP Γ (Pair x y) *)
-  (* | NilP {τ} : ValueP Γ (Nil (τ:=τ)) *)
-  (* | ConsP {τ} (x : Exp Γ τ) xs : *)
-  (*   ValueP Γ x → ValueP Γ xs → ValueP Γ (Cons x xs) *)
+  | LiteralP {ty l} : ValueP Γ (Lit (ty:=ty) l)
+  | BuiltinP {τ b} : ValueP Γ (Bltn (τ:=τ) b)
+  | PairP {τ1 τ2} {x : Exp Γ τ1} {y : Exp Γ τ2} :
+    ValueP Γ x → ValueP Γ y → ValueP Γ (Pair x y)
+  | NilP {τ} : ValueP Γ (Nil (τ:=τ))
+  | ConsP {τ} (x : Exp Γ τ) xs :
+    ValueP Γ x → ValueP Γ xs → ValueP Γ (Cons x xs)
   | LambdaP {dom cod} (e : Exp (dom :: Γ) cod) : ValueP Γ (LAM e).
 
 Derive Signature for ValueP.
@@ -40,42 +36,59 @@ Inductive ErrorP Γ : ∀ {τ}, Exp Γ τ → Prop :=
 
 Derive Signature for ErrorP.
 
+Set Elimination Schemes.
+
+Scheme ValueP_ind := Induction for ValueP Sort Prop.
+Scheme ErrorP_ind := Induction for ErrorP Sort Prop.
+
 #[local] Hint Constructors ValueP ErrorP : core.
 
 Lemma ValueP_irrelevance {Γ τ} (v : Exp Γ τ) (H1 H2 : ValueP _ v) :
   H1 = H2.
 Proof.
-  dependent elimination H1;
-  dependent elimination H2; auto.
+  dependent induction H1;
+  dependent elimination H2; auto;
+  f_equal; congruence.
 Qed.
 
 Lemma ErrorP_irrelevance {Γ τ} (v : Exp Γ τ) (H1 H2 : ErrorP _ v) :
   H1 = H2.
 Proof.
-  dependent elimination H1;
-  dependent elimination H2; auto.
+  dependent induction H1;
+  dependent elimination H2; auto;
+  f_equal; congruence.
 Qed.
 
 Lemma ValueP_dec {Γ τ} (e : Exp Γ τ) :
   ValueP Γ e ∨ ¬ ValueP Γ e.
-Proof. induction e; solve [now left|now right]. Qed.
+Proof.
+  induction e; try solve [now left|now right].
+  - destruct IHe1, IHe2.
+    + now left; constructor.
+    + right; intro; inv H1; contradiction.
+    + right; intro; inv H1; contradiction.
+    + right; intro; inv H1; contradiction.
+  - destruct IHe1, IHe2.
+    + now left; constructor.
+    + right; intro; inv H1; contradiction.
+    + right; intro; inv H1; contradiction.
+    + right; intro; inv H1; contradiction.
+Qed.
 
 Lemma ErrorP_dec {Γ τ} (e : Exp Γ τ) :
   ErrorP Γ e ∨ ¬ ErrorP Γ e.
-Proof. induction e; solve [now left|now right]. Qed.
+Proof.
+  induction e; solve [now left|now right].
+Qed.
 
 End Value.
 
-Arguments ValueP {A H Γ τ} _.
-(* Arguments HostedValP {A H Γ ty} _. *)
-(* Arguments HostedFunP {A H Γ dom cod} _. *)
-(* Arguments ErrorP {A H Γ τ} _. *)
-Arguments UnitP {A H Γ}.
-(* Arguments TrueP {A H Γ}. *)
-(* Arguments FalseP {A H Γ}. *)
-(* Arguments PairP {A H Γ τ1 τ2 x y} _ _. *)
-(* Arguments NilP {A H Γ τ}. *)
-(* Arguments ConsP {A H Γ τ _ _} _ _. *)
-Arguments LambdaP {A H Γ dom cod} _.
+Arguments ValueP {Γ τ} _.
+Arguments LiteralP {Γ}.
+Arguments BuiltinP {Γ}.
+Arguments PairP {Γ τ1 τ2 x y} _ _.
+Arguments NilP {Γ τ}.
+Arguments ConsP {Γ τ _ _} _ _.
+Arguments LambdaP {Γ dom cod} _.
 
-Arguments ErrorP {A H Γ τ} _.
+Arguments ErrorP {Γ τ} _.
