src/Data/Semigroup.v
@@ -22,6 +22,7 @@ Definition Maybe_append `{Semigroup a} (x y : Maybe a) : Maybe a :=
   | Just x, Just y => Just (x ⨂ y)
   end.
 
+#[global]
 Program Instance Semigroup_Maybe `{Semigroup a} : Semigroup (Maybe a) := {
   mappend := Maybe_append
 }.
