src/Sound.v
@@ -42,7 +42,7 @@ Proof.
   (*   specialize (IHe1 _ _ H H4). *)
   (*   apply ExpR_R in IHe1. *)
   (*   unfold denoted in IHe1; reduce. *)
-Admitted.
+Abort.
 
 Theorem Exp_sound {τ} (e e' : Exp [] τ) : e ---> e' → Sound e e'.
 Proof.
